CoqOfRust/core/simulations/clone.v
@@ -1,0 +1,28 @@
+Require Import CoqOfRust.CoqOfRust.
+Require Import proofs.M.
+Require Import simulations.M.
+
+Import Run.
+
+(*
+    pub trait Clone: Sized {
+        fn clone(&self) -> Self;
+
+        fn clone_from(&mut self, source: &Self) {
+            *self = source.clone()
+        }
+    }
+*)
+Module Clone.
+  Record RunImpl `{State.Trait} (Self : Set) `{ToTy Self} `{ToValue Self} : Set := {
+    clone : {clone @
+      IsTraitMethod "core::clone::Clone" (Φ Self) [] "clone" clone *
+      forall (state : State) (pointer : Pointer.t Value.t),
+        HasRead.t state pointer φ ->
+        {{ _, _, state |
+          clone [] [ Value.Pointer pointer ] ⇓ (fun v => inl (φ v))
+        | fun state' => state' = state }}
+    };
+    (* TODO: add [clone_from] *)
+  }.
+End Clone.
